Allocate.v
@@ -1,13 +1,9 @@
-Require Import Coq.Program.Basics.
 Require Import Coq.Structures.Orders.
-Require Import Coq.Vectors.Vector.
-Require Import Compare.
-Require Import Fin.
 Require Import Interval.
 Require Import Lib.
 Require Import ScanState.
-Require Import Vector.
 Require Import SSMorph.
+Require Import Hask.State.
 
 Open Scope program_scope.
 
@@ -15,34 +11,6 @@ Generalizable All Variables.
 
 Module MAllocate (M : Machine).
 Include MSSMorph M.
-
-(** Given a vector of optional positions associated with register, return the
-    first register (counting downwards) which is either [None], or the highest
-    of [Some] value.
-
-    The worst case scenario is that every register has [Some n] with the same
-    n, in which case register 0 is selected. *)
-
-Definition registerWithHighestPos
-  : Vec (option nat) maxReg -> fin maxReg * option nat :=
-  fold_left_with_index
-    (fun reg (res : fin maxReg * option nat) x =>
-       match (res, x) with
-       | ((r, None), _) => (r, None)
-       | (_, None) => (reg, None)
-       | ((r, Some n), Some m) =>
-         if n <? m then (reg, Some m) else (r, Some n)
-       end) (from_nat 0 registers_exist, Some 0).
-
-(** Given a vector from registers to values, find the slot corresponding to
-    the register assigned to [i] and replace it with [x]. *)
-
-Definition atIntervalReg {sd : ScanStateDesc} (i : IntervalId sd)
-  {a} (v : Vec a maxReg) (x : a) :=
-  match V.nth (assignments sd) i with
-  | None => v
-  | Some r => replace v r x
-  end.
 
 (** Split the current interval before the position [before].  This must
     succeed, which means there must be use positions within the interval prior
@@ -55,19 +23,21 @@ Definition atIntervalReg {sd : ScanStateDesc} (i : IntervalId sd)
 
     jww (2014-10-01): Prove that it always succeeds. *)
 
-Definition splitInterval `(cur : ScanStateCursor sd) (before : option nat)
-  : NextState cur SSMorphStLen :=
+Definition SState P :=
+  State { sd : ScanStateDesc & { cur : ScanStateCursor sd & NextState cur P }}.
+
+Definition splitCurrentInterval `(cur : ScanStateCursor sd)
+  (before : option nat) : NextState cur SSMorphStLen :=
   (* jww (2014-09-26): NYI *)
   Build_NextScanState sd (curState cur) undefined.
 
-Definition getInterval `(i : IntervalId sd) :=
-  proj2_sig (V.nth (intervals sd) i).
+Definition splitActiveIntervalForReg `(st : ScanState sd) (reg : PhysReg)
+  (position : nat) : NextScanState (SSMorphLen sd).
+  (* jww (2014-10-01): NYI *)
+Admitted.
 
-Definition getAssignment `(i : IntervalId sd) :=
-  V.nth (assignments sd) i.
-
-Definition assignRegister `(cur : ScanStateCursor sd)
-  (reg : PhysReg) : NextState cur SSMorphLen.
+Definition splitAnyInactiveIntervalForReg `(st : ScanState sd) (reg : PhysReg) :
+  NextScanState (SSMorphLen sd).
   (* jww (2014-10-01): NYI *)
 Admitted.
 
@@ -85,7 +55,7 @@ Definition tryAllocateFreeReg `(cur : ScanStateCursor sd)
        freeUntilPos[it.reg] = next intersection of it with current *)
   let go n := fold_left (fun v i => atIntervalReg i v (n i)) in
   let freeUntilPos' := go (fun _ => Some 0)
-                          (active sd) (const None maxReg) in
+                          (active sd) (V.const None maxReg) in
   let intersectingIntervals :=
       filter (fun x => anyRangeIntersects current (getInterval x))
              (inactive sd) in
@@ -97,6 +67,10 @@ Definition tryAllocateFreeReg `(cur : ScanStateCursor sd)
   (* mres = highest use position of the found register *)
   let (reg, mres) := registerWithHighestPos freeUntilPos in
 
+  (** [moveUnhandledToActive] not only moves an [IntervalId] from the
+      [unhandled] list to the [active] list in the current [ScanStateDesc], it
+      also assignments a register to that newly active interval, which can be
+      accessed by calling [getAssignment]. *)
   let success := moveUnhandledToActive cur reg in
   match mres with
   | None => Some success
@@ -115,8 +89,8 @@ Definition tryAllocateFreeReg `(cur : ScanStateCursor sd)
     then None
     else Some (if intervalEnd current <? n
                then success
-               else let spl    := splitInterval cur (Some n) in
-                    let cur'   := cursorFromMorphStLen cur spl in
+               else let spl  := splitCurrentInterval cur (Some n) in
+                    let cur' := cursorFromMorphStLen cur spl in
                     moveUnhandledToActive cur' reg)
   end.
 
@@ -124,13 +98,17 @@ Definition nextUseAfter `(curId : Interval desc) (pos : nat) : option nat.
   (* jww (2014-09-26): NYI *)
 Admitted.
 
+Definition firstUseReqReg `(curId : Interval desc) : option nat.
+  (* jww (2014-10-01): NYI *)
+Admitted.
+
 Definition assignSpillSlotToCurrent `(cur : ScanStateCursor sd)
   : NextScanState (SSMorphLen sd).
   (* jww (2014-09-26): NYI *)
 Admitted.
 
-Definition intersectsWithFixedInternal `(cur : ScanStateCursor sd)
-  (reg : PhysReg) : bool.
+Definition intersectsWithFixedInterval `(cur : ScanStateCursor sd)
+  (reg : PhysReg) : option nat.
   (* jww (2014-10-01): NYI *)
 Admitted.
 
@@ -139,6 +117,7 @@ Admitted.
     the change to the [ScanState] must be a productive one. *)
 Definition allocateBlockedReg `(cur : ScanStateCursor sd)
   : NextState cur SSMorphSt :=
+  let st      := curState cur in
   let current := curInterval cur in
   let start   := intervalStart current in
   let pos     := curPosition cur in
@@ -148,10 +127,9 @@ Definition allocateBlockedReg `(cur : ScanStateCursor sd)
        nextUsePos[it.reg] = next use of it after start of current
      for each interval it in inactive intersecting with current do
        nextUsePos[it.reg] = next use of it after start of current *)
-  let go :=
-      fold_left (fun v i =>
-                   atIntervalReg i v (nextUseAfter (getInterval i) start)) in
-  let nextUsePos' := go (active sd) (const None maxReg) in
+  let go := fold_left (fun v i =>
+              atIntervalReg i v (nextUseAfter (getInterval i) start)) in
+  let nextUsePos' := go (active sd) (V.const None maxReg) in
   let intersectingIntervals :=
       filter (fun x => anyRangeIntersects current (getInterval x))
              (inactive sd) in
@@ -171,28 +149,48 @@ Definition allocateBlockedReg `(cur : ScanStateCursor sd)
        current.reg = reg
        split active interval for reg at position
        split any inactive interval for reg at the end of its lifetime hole *)
-  let firstUse := undefined in
-  let next :=
-      if (match mres with
-          | None   => false
-          | Some n => n <? firstUse
-          end)
-      then let next := assignSpillSlotToCurrent cur in
-           let firstUseReqReg := undefined in
-           splitInterval cur (Some firstUseReqReg)
-      else undefined in
 
   (* // make sure that current does not intersect with
      // the fixed interval for reg
      if current intersects with the fixed interval for reg then
        split current before this intersection *)
-  let cursor := cursorFromMorphStLen cur next in
-  if intersectsWithFixedInternal cursor reg
-  (* then moveUnhandledToActive *)
-  (*          (cursorFromMorphStLen cursor (splitInterval cursor undefined)) reg *)
-  (* else next. *)
-  then undefined
-  else undefined.
+  if (match mres with
+      | None   => false
+      | Some n => n <? start
+      end)
+  then
+    let n1   := assignSpillSlotToCurrent cur in
+    let cur1 := cursorFromMorphLen cur n1 in
+
+    let n2   := splitCurrentInterval cur1 (firstUseReqReg current) in
+    let cur2 := cursorFromMorphStLen cur1 n2 in
+
+    match intersectsWithFixedInterval cur2 reg with
+    | Some n =>
+        let n3 := splitCurrentInterval cur2 (Some n) in
+        NS_SSMorphSt_Len_StLen_StLen_transitivity cur n1 n2 n3
+    | None => NS_SSMorphSt_Len_StLen_transitivity cur n1 n2
+    end
+  else
+    let n1   := splitActiveIntervalForReg st reg pos in
+    let cur1 := cursorFromMorphLen cur n1 in
+
+    let n2   := splitAnyInactiveIntervalForReg (nextState n1) reg in
+    let cur2 := cursorFromMorphLen cur1 n2 in
+
+    match intersectsWithFixedInterval cur2 reg with
+    | Some n =>
+        let n3   := splitCurrentInterval cur2 (Some n) in
+        let cur3 := cursorFromMorphStLen cur2 n3 in
+        let n4   := @NS_SSMorphStLen_Len_Len_StLen_transitivity
+                      _ cur n1 cur1 n2 cur2 n3 in
+        let cur4 := cursorFromMorphStLen cur n4 in
+        let n5   := moveUnhandledToActive cur4 reg in
+        NS_SSMorphSt_StLen_St_transitivity cur n4 n5
+    | None =>
+        let n3   := moveUnhandledToActive cur2 reg in
+        @NS_SSMorphSt_Len_Len_St_transitivity _ cur n1 cur1 n2 cur2 n3
+    end.
 
 Fixpoint checkActiveIntervals `(st : ScanState sd) pos
   : NextScanState (SSMorphLen sd) :=
@@ -244,20 +242,14 @@ Definition handleInterval `(cur : ScanStateCursor sd)
   let position := curPosition cur in
 
   (* // check for intervals in active that are handled or inactive *)
-  let sp1  := checkActiveIntervals (curState cur) position in
-  let Hlt1 := unhandled_nonempty sd (nextDesc sp1) (morphProof sp1)
-                                 (curExists cur) in
-  let H1   := next_interval_increases (morphProof sp1) in
-  let cid1 := transportId H1 (curId cur) in
+  let n1   := checkActiveIntervals (curState cur) position in
+  let cur1 := cursorFromMorphLen cur n1 in
 
   (* jww (2014-10-01): OPTIONAL Prove: length active <=. *)
 
   (* // check for intervals in inactive that are handled or active *)
-  let sp2  := checkInactiveIntervals (nextState sp1) position in
-  let Hlt2 := unhandled_nonempty (nextDesc sp1) (nextDesc sp2)
-                                 (morphProof sp2) Hlt1 in
-  let H2   := next_interval_increases (morphProof sp2) in
-  let cid2 := transportId H2 cid1 in
+  let n2   := checkInactiveIntervals (nextState n1) position in
+  let cur2 := cursorFromMorphLen cur1 n2 in
 
   (* jww (2014-10-01): OPTIONAL Prove: length inactive <=. *)
 
@@ -267,17 +259,9 @@ Definition handleInterval `(cur : ScanStateCursor sd)
        allocateBlockedReg
      if current has a register assigned then
        add current to active (done by the helper functions) *)
-  let cursor := {| curState  := nextState sp2
-                 ; curExists := Hlt2
-                 |} in
-  let result := fromMaybe (allocateBlockedReg cursor)
-                          (tryAllocateFreeReg cursor) in
-  {| nextDesc   := nextDesc result
-   ; nextState  := nextState result
-   ; morphProof :=
-       SSMorphLenLenSt_transitivity (morphProof sp1) (morphProof sp2)
-                                    (morphProof result)
-   |}.
+  let n3 := fromMaybe (allocateBlockedReg cur2)
+                      (tryAllocateFreeReg cur2) in
+  @NS_SSMorphSt_Len_Len_St_transitivity _ cur n1 cur1 n2 cur2 n3.
 
 Function linearScan (sd : ScanStateDesc) (st : ScanState sd)
   {measure unhandledExtent sd} : { sd' : ScanStateDesc | ScanState sd' } :=
@@ -286,10 +270,9 @@ Function linearScan (sd : ScanStateDesc) (st : ScanState sd)
        HANDLE_INTERVAL (current) *)
   match destruct_list (unhandled sd) with
   | inleft (existT x (exist xs H)) =>
-    let cursor := {| curState  := st
-                   ; curExists := list_cons_nonzero H
-                   |} in
-    match handleInterval cursor with
+    match handleInterval
+            {| curState  := st
+             ; curExists := list_cons_nonzero H |} with
       Build_NextScanState sd2 st2 smorph2 => linearScan sd2 st2
     end
   | inright _ => exist _ sd st
